# **The Equation for A Rectangular Hyperbola And The Equation of The Tangent And The Equation of The Normal**

## Learning Objectives

- Understand the parametric and Cartesian equations of a rectangular hyperbola.
- Learn to derive the equation of the tangent and normal from the equations.

## Teaching Process

### 1. Introduction to Rectangular Hyperbola

- Parametric equations of a rectangular hyperbola: $x=ct$, $y=\frac{c}{t}$, $t\in \mathbb{R}$, $t\neq 0$, $c>0$.
- Cartesian equation of a rectangular hyperbola: $xy=c^2$, $c>0$.
- The curve has asymptotes $x=0$ and $y=0$, which are perpendicular to each other, and the reason why it is called a **rectangular** hyperbola.

### 2. Example 8

#### 8.a

- Rearrange the equation $xy=8$ to the form $y=\frac{8}{x}$.
- Take the derivative to find the tangent slope when $x=2$: $y'=-\frac{8}{x^2}=-2$.
- When $x=2$, $y=4$, so the point of tangency is $(2,4)$.

#### 8.b

- The equation of the tangent line is $y-4=-2(x-2)$, which simplifies to $y=-2x+8$.
- Gradient of tangent at $P$ is $-2$, so the gradient of the normal is $\frac{1}{2}$.
- The equation of the normal line is $y-4=\frac{1}{2}(x-2)$, which simplifies to $2y=x+6$.

### 3. Example 9

#### 9.a

- When $x=3$, $y^2=27\times 3=81$, so $y=\pm 9$. Hence $A$ and $B$ are $(3,9)$ and $(3,-9)$.

#### 9.b

- We can see from the graph that the gradient of $l_1$ is positive, and the gradient of $l_2$ is negative.

#### 9.c

- Since $y=\pm3\sqrt{3}x^{\frac{1}{2}}$, the derivative is $y'=\pm\frac{3}{2}\sqrt{3}x^{-\frac{1}{2}}$.
- The gradient of the tangent line $l_1$ at $A$ is $\frac{3\sqrt{3}}{2\sqrt{3}}=\frac{3}{2}$.
- With point $A(3,9)$ and gradient $\frac{3}{2}$, the equation of the tangent line is $y-9=\frac{3}{2}(x-3)$, which simplifies to $3x-2y+9=0$. 
- The gradient of the tangent line $l_2$ at $B$ is $-\frac{3}{2}$.
- With point $B(3,-9)$ and gradient $-\frac{3}{2}$, the equation of the tangent line is $y+9=-\frac{3}{2}(x-3)$, which simplifies to $3x+2y+9=0$.

### 4. Example 10

- Since $y^2=12x$, and $y_P=6$, we have $y=\sqrt{12x}$.
- The derivative is $y'=2\sqrt{3}\left(\frac{1}{2}\right)x^{-\frac{1}{2}}$.
- The gradient of the tangent line at $P$ is $\frac{2\sqrt{3}}{2\sqrt{3}}=1$.
- With point $P(3,6)$ and gradient $1$, the equation of the tangent line is $y-6=1(x-3)$, which simplifies to $x-y+3=0$.